formal/inference/heuristics/Store_Reuse_Subsumption.thy
@@ -683,4 +683,49 @@ lemma input_stored_in_reg_updates_reg: "input_stored_in_reg t2 t1 a = Some (i, r
   apply simp
   by (simp add: is_generalisation_of_def remove_guard_add_update_def)
 
+definition "possibly_not_value_ctx v r t\<^sub>1 s\<^sub>2 e\<^sub>2 s\<^sub>1 e\<^sub>1 =
+  (\<exists>p. accepts_trace (tm e\<^sub>1) p \<and> gets_us_to s\<^sub>1 (tm e\<^sub>1) 0 <>  p \<and>
+       accepts_trace (tm e\<^sub>2) p \<and> gets_us_to s\<^sub>2 (tm e\<^sub>2) 0 <> p \<and>
+       (case anterior_context (tm e\<^sub>2) p of None \<Rightarrow> False | Some c \<Rightarrow>
+       (\<exists>i. can_take_transition t\<^sub>1 i c) \<and>
+       c $ r \<noteq> Some v)
+  )"
+
+lemma possibly_not_value: 
+  "stored_reused t\<^sub>2 t\<^sub>1 = Some (r, p) \<Longrightarrow>
+   nth (Outputs t\<^sub>1) p = L v \<Longrightarrow>
+   p < length (Outputs t\<^sub>1) \<Longrightarrow>
+   possibly_not_value_ctx v r t\<^sub>1 s\<^sub>2 e\<^sub>2 s\<^sub>1 e\<^sub>1 \<Longrightarrow>
+   \<not> directly_subsumes e\<^sub>1 e\<^sub>2 s\<^sub>1 s\<^sub>2 t\<^sub>2 t\<^sub>1"
+  apply (simp add: directly_subsumes_def possibly_not_value_ctx_def)
+  apply (rule disjI1)
+  apply clarify
+  apply (rule_tac x=pa in exI)
+  apply clarify
+  apply (case_tac "anterior_context (tm e\<^sub>2) pa")
+  apply simp
+  apply simp
+  using stored_reused_is_generalised_output_of[of t\<^sub>2 t\<^sub>1 r p]
+  using is_generalised_output_of_does_not_subsume[of t\<^sub>2 t\<^sub>1 r p v]
+  by auto
+
+definition "possibly_not_value e\<^sub>1 e\<^sub>2 s\<^sub>1 s\<^sub>2 t\<^sub>2 t\<^sub>1 =
+  (case stored_reused t\<^sub>2 t\<^sub>1 of None \<Rightarrow> False | Some (r, p) \<Rightarrow>
+    (case nth (Outputs t\<^sub>1) p of L v \<Rightarrow>
+      p < length (Outputs t\<^sub>1) \<and>
+      possibly_not_value_ctx v r t\<^sub>1 s\<^sub>2 e\<^sub>2 s\<^sub>1 e\<^sub>1 |
+    _ \<Rightarrow> False)
+  )"
+
+lemma possibly_not_value_not_directly_subsumes: 
+  "possibly_not_value e\<^sub>1 e\<^sub>2 s\<^sub>1 s\<^sub>2 t\<^sub>2 t\<^sub>1 \<Longrightarrow> \<not> directly_subsumes e\<^sub>1 e\<^sub>2 s\<^sub>1 s\<^sub>2 t\<^sub>2 t\<^sub>1"
+  apply (simp add: possibly_not_value_def)
+  apply (case_tac "stored_reused t\<^sub>2 t\<^sub>1")
+   apply simp
+  apply (case_tac a)
+  apply simp
+  apply (case_tac "Outputs t\<^sub>1 ! b")
+     apply (simp add: possibly_not_value)
+  by auto
+
 end
